Tweak in for_wpl; CP in adding for_elab

examples/refinement/HighComp.fst
@@ -97,19 +97,21 @@ let ite_wp #a (b : bool) (wp1 : hwp a{monotonic wp1})
   (wp2 : hwp a{monotonic wp2}) : wp:hwp a{monotonic wp} = 
   HIGH?.wp_if_then_else a b wp1 wp2  
 
-val wp_for : (int -> hwp_mon unit) -> (lo : int) -> (hi : int{hi >= lo}) -> Tot (hwp_mon unit) (decreases (hi - lo))
-let rec wp_for (wp:int -> hwp_mon unit) (lo : int) (hi : int{hi >= lo}) : Tot (hwp_mon unit) (decreases (hi - lo)) = 
+val for_wp : (int -> hwp_mon unit) -> (lo : int) -> (hi : int{hi >= lo}) -> Tot (hwp_mon unit) (decreases (hi - lo))
+let rec for_wp (wp:int -> hwp_mon unit) (lo : int) (hi : int{hi >= lo}) : Tot (hwp_mon unit) (decreases (hi - lo)) = 
   if lo = hi then (return_wp ())
-  else 
-    (fun s0 post -> 
-       wp lo s0 (fun ((), s1) ->
-       wp_for wp (lo + 1) hi s1 post))
+  else (bind_wp (wp lo) (fun (_:unit) -> for_wp wp (lo + 1) hi))
+    // (fun s0 post -> 
+    //    wp lo s0 (fun ((), s1) ->
+    //    wp_for wp (lo + 1) hi s1 post))
   
 // for combinator
-let rec for (#wp : int -> hwp_mon unit) (lo : int) (hi : int{lo <= hi}) (f : (i:int) -> HIGH unit (wp i)) : HIGH unit (wp_for wp lo hi) (decreases (hi - lo)) =
+let rec for (#wp : int -> hwp_mon unit) (lo : int) (hi : int{lo <= hi}) (f : (i:int) -> HIGH unit (wp i)) :
+    HIGH unit (for_wp wp lo hi) (decreases (hi - lo)) =
   if lo = hi then ()
   else 
-    (f lo; for #wp (lo + 1) hi f)
+  (f lo; for #wp (lo + 1) hi f)
+
 
 // Pre and postconditions
 
@@ -131,6 +133,13 @@ let return_elab (#a:Type) (x : a) : comp_wp a (return_wp x) =
   HIGH?.return_elab a x
 
 let bind_elab #a #b #f_w ($f:_) #g_w ($g:_) : comp_wp b (bind_wp f_w g_w) = HIGH?.bind_elab a b f_w f g_w g
+
+
+// let rec for_elab (#wp : int -> hwp_mon unit) (lo : int) (hi : int{lo <= hi}) (f : (i:int) -> comp_wp unit (wp i)) : 
+//     comp_wp unit (wp_for wp lo hi) (decreases (hi - lo)) =
+//   if lo = hi then (return_elab ())
+//   else (bind_elab (f lo) (fun (_ : unit) -> for_elab #wp (lo + 1) hi f))
+
 
 val hread' : i:nat -> comp_wp mint (read_wp i)
 let hread' (i:nat) : comp_wp mint (read_wp i) =
